src/HOL/Hoare/Examples.thy
@@ -6,4 +6,207 @@
 Various examples.
 *)
 
-Examples = Hoare + Arith2
+theory Examples = Hoare + Arith2:
+
+(*** ARITHMETIC ***)
+
+(** multiplication by successive addition **)
+
+lemma multiply_by_add: "|- VARS m s a b.
+  {a=A & b=B}
+  m := 0; s := 0;
+  WHILE m~=a
+  INV {s=m*b & a=A & b=B}
+  DO s := s+b; m := m+(1::nat) OD
+  {s = A*B}"
+by vcg_simp
+
+
+(** Euclid's algorithm for GCD **)
+
+lemma Euclid_GCD: "|- VARS a b.
+ {0<A & 0<B}
+ a := A; b := B;
+ WHILE  a~=b
+ INV {0<a & 0<b & gcd A B = gcd a b}
+ DO IF a<b THEN b := b-a ELSE a := a-b FI OD
+ {a = gcd A B}"
+apply vcg
+(*Now prove the verification conditions*)
+  apply auto
+  apply(simp add: gcd_diff_r less_imp_le)
+ apply(simp add: not_less_iff_le gcd_diff_l)
+apply(erule gcd_nnn)
+done
+
+(** Dijkstra's extension of Euclid's algorithm for simultaneous GCD and SCM **)
+(* From E.W. Disjkstra. Selected Writings on Computing, p 98 (EWD474),
+   where it is given without the invariant. Instead of defining scm
+   explicitly we have used the theorem scm x y = x*y/gcd x y and avoided
+   division by mupltiplying with gcd x y.
+*)
+
+lemmas distribs =
+  diff_mult_distrib diff_mult_distrib2 add_mult_distrib add_mult_distrib2
+
+lemma gcd_scm: "|- VARS a b x y.
+ {0<A & 0<B & a=A & b=B & x=B & y=A}
+ WHILE  a ~= b
+ INV {0<a & 0<b & gcd A B = gcd a b & 2*A*B = a*x + b*y}
+ DO IF a<b THEN (b := b-a; x := x+y) ELSE (a := a-b; y := y+x) FI OD
+ {a = gcd A B & 2*A*B = a*(x+y)}"
+apply vcg
+  apply simp
+ apply(simp add: distribs gcd_diff_r not_less_iff_le gcd_diff_l)
+ apply arith
+apply(simp add: distribs gcd_nnn)
+done
+
+(** Power by iterated squaring and multiplication **)
+
+lemma power_by_mult: "|- VARS a b c.
+ {a=A & b=B}
+ c := (1::nat);
+ WHILE b ~= 0
+ INV {A^B = c * a^b}
+ DO  WHILE b mod 2 = 0
+     INV {A^B = c * a^b}
+     DO  a := a*a; b := b div 2 OD;
+     c := c*a; b := b - 1
+ OD
+ {c = A^B}"
+apply vcg_simp
+apply(case_tac "b")
+ apply(simp add: mod_less)
+apply simp
+done
+
+(** Factorial **)
+
+lemma factorial: "|- VARS a b.
+ {a=A}
+ b := 1;
+ WHILE a ~= 0
+ INV {fac A = b * fac a}
+ DO b := b*a; a := a - 1 OD
+ {b = fac A}"
+apply vcg_simp
+apply(clarsimp split: nat_diff_split)
+done
+
+
+(** Square root **)
+
+(* the easy way: *)
+
+lemma sqrt: "|- VARS r x.
+ {True}
+ x := X; r := (0::nat);
+ WHILE (r+1)*(r+1) <= x
+ INV {r*r <= x & x=X}
+ DO r := r+1 OD
+ {r*r <= X & X < (r+1)*(r+1)}"
+apply vcg_simp
+apply auto
+done
+
+(* without multiplication *)
+
+lemma sqrt_without_multiplication: "|- VARS u w r x.
+ {True}
+ x := X; u := 1; w := 1; r := (0::nat);
+ WHILE w <= x
+ INV {u = r+r+1 & w = (r+1)*(r+1) & r*r <= x & x=X}
+ DO r := r + 1; w := w + u + 2; u := u + 2 OD
+ {r*r <= X & X < (r+1)*(r+1)}"
+apply vcg_simp
+apply auto
+done
+
+
+(*** LISTS ***)
+
+lemma imperative_reverse: "|- VARS y x.
+ {x=X}
+ y:=[];
+ WHILE x ~= []
+ INV {rev(x)@y = rev(X)}
+ DO y := (hd x # y); x := tl x OD
+ {y=rev(X)}"
+apply vcg_simp
+ apply(simp add: neq_Nil_conv)
+ apply auto
+done
+
+lemma imperative_append: "|- VARS x y.
+ {x=X & y=Y}
+ x := rev(x);
+ WHILE x~=[]
+ INV {rev(x)@y = X@Y}
+ DO y := (hd x # y);
+    x := tl x
+ OD
+ {y = X@Y}"
+apply vcg_simp
+apply(simp add: neq_Nil_conv)
+apply auto
+done
+
+
+(*** ARRAYS ***)
+
+(* Search for a key *)
+lemma zero_search: "|- VARS A i.
+ {True}
+ i := 0;
+ WHILE i < length A & A!i ~= key
+ INV {!j. j<i --> A!j ~= key}
+ DO i := i+1 OD
+ {(i < length A --> A!i = key) &
+  (i = length A --> (!j. j < length A --> A!j ~= key))}"
+apply vcg_simp
+apply(blast elim!: less_SucE)
+done
+
+(* 
+The `partition' procedure for quicksort.
+`A' is the array to be sorted (modelled as a list).
+Elements of A must be of class order to infer at the end
+that the elements between u and l are equal to pivot.
+
+Ambiguity warnings of parser are due to := being used
+both for assignment and list update.
+*)
+lemma lem: "m - Suc 0 < n ==> m < Suc n"
+by arith
+
+
+lemma Partition:
+"[| leq == %A i. !k. k<i --> A!k <= pivot;
+    geq == %A i. !k. i<k & k<length A --> pivot <= A!k |] ==>
+ |- VARS A u l.
+ {0 < length(A::('a::order)list)}
+ l := 0; u := length A - Suc 0;
+ WHILE l <= u
+  INV {leq A l & geq A u & u<length A & l<=length A}
+  DO WHILE l < length A & A!l <= pivot
+     INV {leq A l & geq A u & u<length A & l<=length A}
+     DO l := l+1 OD;
+     WHILE 0 < u & pivot <= A!u
+     INV {leq A l & geq A u  & u<length A & l<=length A}
+     DO u := u - 1 OD;
+     IF l <= u THEN A := A[l := A!u, u := A!l] ELSE SKIP FI
+  OD
+ {leq A u & (!k. u<k & k<l --> A!k = pivot) & geq A l}"
+(* expand and delete abbreviations first *)
+apply (simp);
+apply (erule thin_rl)+
+apply vcg_simp
+    apply (force simp: neq_Nil_conv)
+   apply (blast elim!: less_SucE intro: Suc_leI)
+  apply (blast elim!: less_SucE intro: less_imp_diff_less dest: lem)
+ apply (force simp: nth_list_update)
+apply (auto intro: order_antisym)
+done
+
+end
